src/core/Ty.v
@@ -1,6 +1,576 @@
+Require Import Wstdlib.
+Require Import Ident.
+Require Number.
+Require Import stdpp.base.
+Require Import Coq.Wellfounded.Inverse_Image.
 
-(*Temp*)
-Require Export Ident.
+Record tvsymbol := {
+  tv_name : ident
+}.
+
+Definition tvsymbol_eqb (t1 t2: tvsymbol) : bool :=
+  ident_eqb t1.(tv_name) t2.(tv_name).
+
+Lemma tvsymbol_eqb_eq (t1 t2: tvsymbol): t1 = t2 <-> tvsymbol_eqb t1 t2.
+Proof.
+  unfold tvsymbol_eqb.
+  rewrite <- ident_eqb_eq.
+  destruct t1 as [t1]; destruct t2 as [t2]; simpl;
+  split; intros Heq; inversion Heq; subst; reflexivity.
+Qed.
+
+Definition tvsymbol_eq : base.EqDecision tvsymbol :=
+  dec_from_eqb _ tvsymbol_eqb_eq.
+
+Module TvarTagged <: TaggedType.
+Definition t := tvsymbol.
+Definition tag tv := tv.(tv_name).(id_tag).
+Definition eq := tvsymbol_eq.
+
+End TvarTagged.
+
+Module Tvar := MakeMSH TvarTagged.
+Module Stv := Tvar.S.
+Module Mtv := Tvar.M.
+(*Module Htv := Tvar.H*)
+
+(*== in OCaml*)
+Definition tv_equal (t1 t2: tvsymbol) : bool := tvsymbol_eqb t1 t2.
+Definition tv_hash tv := id_hash tv.(tv_name).
+(*Skip tv_compare*)
+
+(*Not stateful, unlike OCaml*)
+Definition create_tvsymbol (n: preid) : ctr tvsymbol :=
+  i ← id_register n;
+  ctr_ret {| tv_name := i|}.
+
+(*In OCaml, this is a stateful function that stores variables
+  in hash table and looks up to see if any have been
+  created with same name already.
+  Here, we just give a new one - NOTE: is this a problem?*)
+Definition tv_of_string (s: string) : ctr tvsymbol :=
+  create_tvsymbol (id_fresh s).
+
+(** Type Symbols and Types **)
+(*For Now*)
+Unset Elimination Schemes.
+
+
+Inductive type_def_ (A: Type) : Type :=
+  | NoDef_
+  | Alias_: A -> type_def_ A
+  | Range_: Number.int_range -> type_def_ A
+  | Float_: Number.float_format -> type_def_ A.
+
+Record ty_ (A: Type) := 
+  { ty_node: A;
+    ty_tag: CoqBigInt.t}.
+
+Arguments ty_ {A}.
+Arguments ty_node {A}.
+Arguments ty_tag {A}.
+
+Record tysymbol_ (A: Type) := {
+  ts_name : ident;
+  ts_args : list tvsymbol;
+  ts_def : type_def_ (@ty_ A)
+}.
+
+Arguments tysymbol_ {A}.
+Arguments ts_name {A}.
+Arguments ts_args {A}.
+Arguments ts_def {A}.
+
+Inductive ty_node__ : Type :=
+  | Tyvar_ : tvsymbol -> ty_node__
+  | Tyapp_ : @tysymbol_ ty_node__ -> list (@ty_ ty_node__) -> ty_node__.
+
+Definition ty' := @ty_ ty_node__.
+
+Definition tysymbol' := @tysymbol_ ty_node__.
+
+Inductive type_def : Type :=
+  | NoDef
+  | Alias : ty -> type_def
+  | Range: Number.int_range -> type_def
+  | Float: Number.float_format -> type_def
+with ty : Type :=
+  | mk_ty : ty_node_ -> CoqBigInt.t -> ty
+with tysymbol : Type :=
+  | mk_ts : ident -> list tvsymbol -> type_def -> tysymbol
+with ty_node_ : Type :=
+  | Tyvar : tvsymbol -> ty_node_
+  | Tyapp: tysymbol -> list ty -> ty_node_.
+
+
+
+(*Try again*)
+(*
+
+(*This is surprisingly difficult to deal with, because 
+  Coq does not support mixed Record and Inductive mutually
+  recursive types (why3 uses these extensively).
+  We want to mantain compatibility with the API, as external
+  clients like Frama-C do in fact use record notation on these
+  values. 
+  There is a way to encode this by making the recursive argument
+  polymorphic and instantiating it later with itself.
+  This results in the OCaml types we expect, at the cost of
+  being able to write Fixpoint functions, since Coq can no
+  longer tell such definitions are well-founded.
+  We can fix this by defining a size metric and doing
+  well-founded recursion (as in Well-Founded Recursion
+  Done Right). But this is painful to do for every function,
+  and generic functions (say, an induction principle)*)
+
+Inductive type_def (A: Type) : Type :=
+  | NoDef
+  | Alias: A -> type_def A
+  | Range: Number.int_range -> type_def A
+  | Float: Number.float_format -> type_def A.
+
+(*We do this to get around the restriction that
+  Coq Records and Inductives cannot be mutually recursive
+  with each other. TODO: see if we can ensure that
+  this satisfies the correct .mli file*)
+Record ty_ (A: Type) := 
+  { ty_node: A;
+    ty_tag: CoqBigInt.t}.
+
+Arguments ty_ {A}.
+Arguments ty_node {A}.
+Arguments ty_tag {A}.
+
+Record tysymbol_ (A: Type) := {
+  ts_name : ident;
+  ts_args : list tvsymbol;
+  ts_def : type_def (@ty_ A)
+}.
+
+Arguments tysymbol_ {A}.
+Arguments ts_name {A}.
+Arguments ts_args {A}.
+Arguments ts_def {A}.
+
+Inductive ty_node_ : Type :=
+  | Tyvar : tvsymbol -> ty_node_
+  | Tyapp : @tysymbol_ ty_node_ -> list (@ty_ ty_node_) -> ty_node_.
+
+Definition ty := @ty_ ty_node_.
+
+Definition tysymbol := @tysymbol_ ty_node_.
+
+(*This encoding satisfies the expected OCaml interface
+  (with a mixed record-inductive type), but because Coq
+  does not allow us to write this directly, we do not
+  have a good induction principle. While we could
+  (and TODO maybe will) prove an induction principle,
+  we instead give a simpler construction for writing
+  the kinds of functions we will need: those that
+  take a [ty] and match on the [ty_node].
+  First, we need well-foundedness, so we define a size*)
+Section TyFuncs.
+
+Section TySize.
+
+
+(*TODO: try with Xavier trick (Equations bad extraction I think) and manual rec*)
+(*Define size*)
+Fixpoint ty_node_size (t: ty_node_) : nat :=
+  match t with
+  | Tyvar v => 1
+  | Tyapp ts tys => 1 +
+    (*tysymbol size*)
+    (1 + match (ts_def ts) with
+          | NoDef _ => 0
+          | Alias _ x => 1 + (1 + ty_node_size (x.(ty_node)))
+          | _=> 1
+    end) +
+  
+   list_sum 
+      (map (fun (x: ty) => 1 + ty_node_size (x.(ty_node))) tys)
+  end.
+
+Definition ty_size (t: ty) : nat :=
+  1 + ty_node_size (t.(ty_node)).
+
+Definition tysymbol_size (ts: tysymbol) : nat :=
+  1 + match ts_def ts with
+    | NoDef _ => 0
+    | Alias _ x => 1 + ty_size x
+    | _ => 1
+  end.
+
+Lemma ty_node_size_rewrite (t: ty_node_) :
+  ty_node_size t =
+  match t with
+  | Tyvar v => 1
+  | Tyapp ts tys => 1 + tysymbol_size ts + 
+    list_sum (map ty_size tys)
+  end.
+Proof.
+  destruct t; simpl; auto.
+Qed.
+
+Definition ty_size_rel (t1 t2: ty) : Prop :=
+  ty_size t1 < ty_size t2.
+
+Lemma ty_size_rel_wf: well_founded ty_size_rel.
+Proof.
+  unfold well_founded. intros.
+  unfold ty_size_rel.
+  apply Inverse_Image.Acc_inverse_image.
+  apply lt_wf.
+Qed.
+
+Definition ty_node_size_rel (t1 t2: ty) : Prop :=
+  ty_node_size (t1.(ty_node)) < ty_node_size (t2.(ty_node)).
+
+Lemma ty_node_size_rel_wf: well_founded ty_node_size_rel.
+Proof.
+  unfold well_founded. intros.
+  unfold ty_node_size_rel.
+  apply Inverse_Image.Acc_inverse_image.
+  apply lt_wf.
+Qed.
+
+End TySize.
+
+(*Obligations for function def:*)
+
+Lemma node_lt_ty (t: ty):
+  ty_node_size (ty_node t) < ty_size t.
+Proof.
+  unfold ty_size. lia.
+Qed.
+
+Lemma in_tys_lt_app {t ts tys}:
+  ty_node_size (Tyapp ts tys) < ty_size t ->
+  Forall (fun x => ty_size_rel x t) tys.
+Proof.
+  rewrite ty_node_size_rewrite. intros.
+  intros.
+  rewrite List.Forall_forall; intros x Hinx.
+  unfold ty_size_rel.
+  pose proof (in_split x tys Hinx) as Hsplit.
+  destruct Hsplit as [l1 [l2 Htys]]; subst.
+  revert H.
+  rewrite map_app. simpl map.
+  rewrite list_sum_app. simpl list_sum.
+  intros.
+  unfold ty_size at 1. lia.
+Qed.
+
+Section TyBuildSimpl.
+
+Variable (A: Type)(B: Type).
+
+Variable (Hvar: tvsymbol -> A).
+Variable (Happ: tysymbol -> list ty -> B -> A).
+
+Variable (base: B).
+Variable (combine: A -> B -> B).
+
+Fixpoint ty_build_simpl' (t: ty) (ACC: Acc ty_size_rel t) {struct ACC} : A :=
+  match t.(ty_node) as n return ty_node_size n < ty_size t -> A with
+  | Tyvar v => fun _ => Hvar v
+  | Tyapp ts tys => fun Hlt => Happ ts tys
+    ((fix tys_fold (l: list ty) (Hall: Forall (fun x => ty_size_rel x t) l) : B :=
+      match l as l' return Forall (fun x => ty_size_rel x t) l' -> B with
+      | nil => fun _ => base
+      | x :: xs => fun Hall => 
+        combine (ty_build_simpl' x (Acc_inv ACC _ (Forall_inv Hall))) 
+        (tys_fold xs (Forall_inv_tail Hall))
+      end Hall) tys (in_tys_lt_app  Hlt))
+  end (node_lt_ty t).
+
+Definition ty_build_simpl t := ty_build_simpl' t (ty_size_rel_wf t).
+
+(*One theorem we need for using this:*)
+
+Lemma ty_size_rel_node_rel (t1 t2: ty):
+  ty_size_rel t1 t2 <-> ty_node_size_rel t1 t2.
+Proof.
+  unfold ty_size_rel, ty_size, ty_node_size_rel. lia.
+Qed.
+
+Lemma ty_build_simpl_irrel t ACC1 ACC2:
+  ty_build_simpl' t ACC1 = ty_build_simpl' t ACC2.
+Proof.
+  induction t using (well_founded_induction ty_node_size_rel_wf).
+  destruct ACC1; destruct ACC2.
+  simpl.
+  destruct t as [n tg]; simpl. destruct n; auto.
+  f_equal.
+  generalize dependent (in_tys_lt_app (node_lt_ty {| ty_node := Tyapp t l; ty_tag := tg |})).
+  generalize dependent {| ty_node := Tyapp t l; ty_tag := tg |}.
+  induction l; simpl; auto.
+  intros. erewrite IHl. f_equal.
+  apply H.
+  inversion f; subst.
+  apply ty_size_rel_node_rel. auto.
+  auto.
+Qed.
+
+(*And the rewrite lemma:*)
+Lemma ty_build_simpl_rewrite (t: ty) :
+  ty_build_simpl t =
+  match t.(ty_node) with
+        | Tyvar v => Hvar v
+        | Tyapp ts tys => Happ ts tys 
+            (fold_right (fun x acc => combine (ty_build_simpl x) acc) base tys)
+  end.
+Proof.
+  unfold ty_build_simpl at 1.
+  generalize dependent (ty_size_rel_wf t).
+  intros a. destruct a.
+  destruct t as [n tg].
+  destruct n; [reflexivity |].
+  simpl. f_equal.
+  (*Problem: have l in Forall*)
+  generalize dependent (in_tys_lt_app (node_lt_ty {| ty_node := Tyapp t l; ty_tag := tg |})).
+  generalize dependent {| ty_node := Tyapp t l; ty_tag := tg |}.
+  intros t' a'.
+  induction l; simpl; auto.
+  intros.
+  rewrite IHl.
+  f_equal.
+  apply ty_build_simpl_irrel.
+Qed.
+
+End TyBuildSimpl.
+
+(*More general functions*)
+
+(*Do same with Type so that we can write functions and test extraction*)
+
+Definition type_def_p_ty (P: ty -> Type) (t: type_def ty_) : Type :=
+  match t with
+  | Alias _ x => P x
+  | _ => True
+  end.
+
+
+Inductive ForallT {A: Type} (P: A -> Type) : list A -> Type :=
+  | ForallT_nil: ForallT P nil
+  | ForallT_cons: forall {x: A} {l: list A},
+    P x -> ForallT P l -> ForallT P (x :: l).
+
+Lemma ForallT_hd {A: Type} (P: A -> Type) (x: A) (l: list A):
+  ForallT P (x :: l) ->
+  P x.
+Proof.
+  intros. inversion X; subst. apply X0.
+Qed.
+
+Lemma ForallT_tl {A: Type} (P: A -> Type) (x: A) (l: list A):
+  ForallT P (x :: l) ->
+  ForallT P l.
+Proof.
+  intros. inversion X; auto.
+Qed.
+
+Lemma ForallT_In {A: Type} (P: A -> Type)
+  (eq_dec: forall (x y: A), {x = y} + {x <> y}) (l: list A):
+  ForallT P l ->
+  forall x, In x l -> P x.
+Proof.
+  intros Hall. induction Hall; simpl; intros.
+  destruct H.
+  destruct (eq_dec x x0); subst; auto.
+  apply IHHall. destruct H; subst; auto.
+  contradiction.
+Qed.
+
+Lemma typesym_lt_node (ts: tysymbol) (tys: list ty):
+  tysymbol_size ts < ty_node_size (Tyapp ts tys).
+Proof.
+  rewrite ty_node_size_rewrite.
+  lia.
+Qed.
+
+
+Section TyRect.
+
+Variable (P: ty -> Type).
+Variable (P1: ty_node_ -> Type).
+Variable (P2: tysymbol -> Type).
+
+Variable (Hty: forall (t: ty), P1 (t.(ty_node)) -> P t).
+Variable (Hsym: forall (ts: tysymbol), type_def_p_ty P (ts.(ts_def)) ->
+  P2 ts).
+Variable (Hvar: forall v, P1 (Tyvar v)).
+Variable (Happ: forall ts tys, P2 ts -> ForallT P tys -> P1 (Tyapp ts tys)).
+
+(*This does NOT work - tysymbol is not recursive so we can't have
+  a fixpoint on it
+  Maybe could do same trick (assume we have proof, populate later)
+  but likely to run into positivity problems*)
+
+
+(*Fixpoint gcd_rec (a b: nat) (ACC: Acc lt b) {struct ACC} : nat :=
+  if Nat.eq_dec b 0 then a else gcd_rec b (a mod b) (Acc_inv ACC _).*)
+
+(*TODO: need decomposition if we want idiomatic code, maybe need eq_rect*)
+(*Plan: prove lemmas, do in Set, test extraction (without Program) *)
+Fixpoint ty_rect' (t: ty) (ACC: Acc lt (ty_size t)) {struct ACC} : P t :=
+  (Hty t (ty_node_rect' t.(ty_node) 
+    (Acc_inv ACC (ty_node_size (ty_node t)) (node_lt_ty t))))
+with ty_node_rect' (t: ty_node_) (ACC: Acc lt (ty_node_size t)) {struct ACC} : P1 t :=
+  match t as t' return Acc lt (ty_node_size t') -> P1 t' with
+  | Tyvar tv => fun _ => Hvar tv
+  | Tyapp ts tys => fun ACC => Happ ts tys (tysymbol_rect' ts (Acc_inv ACC (tysymbol_size ts) 
+      (typesym_lt_node ts tys))) 
+    ((fix tys_rect (l: list ty) 
+      (Hl: Forall (fun x => ty_size x < (ty_node_size (Tyapp ts tys))) l) 
+      : ForallT P l :=
+      match l as l' return Forall  (fun x => ty_size x < (ty_node_size (Tyapp ts tys))) l'->
+        ForallT P l'  with
+      | nil => fun _ => ForallT_nil _
+      | x :: xs => fun Hl => ForallT_cons _ (ty_rect' x (Acc_inv ACC (ty_size x) 
+        (List.Forall_inv Hl))) 
+        (tys_rect xs (List.Forall_inv_tail Hl))
+      end Hl) tys (in_tys_lt_app ts tys))
+  end ACC
+with tysymbol_rect' (ts: tysymbol) (ACC: Acc lt (tysymbol_size ts)) {struct ACC} : P2 ts :=
+  Hsym ts (
+    match (ts.(ts_def)) as d' return type_def_size d' < tysymbol_size ts -> 
+       type_def_p_ty P d' with
+    | NoDef _ => fun _ => I
+    | Alias _ x => fun Hlt => ty_rect' x (Acc_inv ACC (ty_size x) (alias_lt_sym Hlt))
+    end (def_lt_sym ts)
+  ).
+
+Definition ty_rect (t: ty) : P t := ty_rect' t (lt_wf _).
+Definition ty_node_rect (t: ty_node_) : P1 t := ty_node_rect' t (lt_wf _).
+Definition tysymbol_rect (ts: tysymbol) : P2 ts := tysymbol_rect' ts (lt_wf _).
+
+End TyRect.
+
+(*Example (TODO move)*)
+Definition ty_v_map (f: tvsymbol -> ty) (t: ty) : ty :=
+  ty_build_simpl ty (list ty) (fun v => f v)
+  (fun ts tys res => Build_ty_ _ (Tyapp ts res) CoqBigInt.zero) 
+  nil cons t.
+Print type_def.
+
+(*For equality, we have to do things manually*)
+Fixpoint ty_eqb (t1 t2: ty) (ACC: Acc ty_size_rel t1) {struct ACC} :=
+  ty_node_eqb t1.(ty_node) t2.(ty_node) &&
+  CoqBigInt.eq t1.(ty_tag) t2.(ty_tag) 
+with ty_node_eqb (t1 t2: ty_node) (ACC: Acc ty_node_size_rel t1) {struct ACC} :=
+  match t1, t2 with
+  | Tyvar v1, Tyvar v2 => tvsymbol_eqb v1 v2
+  | Tyapp ts1 tys1, Tyapp ts2 tys2 =>
+    tysymbol_eqb ts1 ts2 &&
+    ((fix tys_eqb (l1 l2: list ty) : bool :=
+      match l1, l2 with
+      | h1 :: tl1, h2 :: tl2 => ty_eqb h1 h2 && tys_eqb tl1 tl2
+      | nil, nil => true
+      | _, _ => false
+      end) tys1 tys2)
+  | _, _ => false
+  end
+with tysymbol_eqb (ts1 ts2: tysymbol) (ACC: Acc tysymbol_size_rel t1) {struct ACC} :=
+  ident_eqb t1.(ts_name) t2.(ts_name) &&
+  list_eqb tvsymbol_eqb t1.(ts_args) t2.(ts_args) &&
+
+
+
+
+Record ty_ (A: Type) := 
+  { ty_node: A;
+    ty_tag: CoqBigInt.t}.
+
+
+
+Fixpoint ty_build_simpl' (t: ty) (ACC: Acc ty_size_rel t) {struct ACC} : A :=
+  match t.(ty_node) as n return ty_node_size n < ty_size t -> A with
+  | Tyvar v => fun _ => Hvar v
+  | Tyapp ts tys => fun Hlt => Happ ts tys
+    ((fix tys_fold (l: list ty) (Hall: Forall (fun x => ty_size_rel x t) l) : B :=
+      match l as l' return Forall (fun x => ty_size_rel x t) l' -> B with
+      | nil => fun _ => base
+      | x :: xs => fun Hall => 
+        combine (ty_build_simpl' x (Acc_inv ACC _ (Forall_inv Hall))) 
+        (tys_fold xs (Forall_inv_tail Hall))
+      end Hall) tys (in_tys_lt_app  Hlt))
+  end (node_lt_ty t).
+
+
+(*This almost works, but not quite, because our function
+  schema is not specific enough*)
+(*Definition ty_eqb (t1 t2: ty) : bool :=
+  (ty_build_simpl (ty -> bool) (list ty -> bool) (fun v t2 => 
+    match t2.(ty_node) with
+    | Tyvar v2 => typevar_eqb v v2
+    | _ => false
+    end) 
+    (fun ts tys res t2 => match t2.(ty_node) with
+    | Tyapp ts1 tys2 => tysymbol_eqb ts ts1 &&
+      res tys2
+    | _ => false
+    end) 
+    (*Base*)
+    (fun l =>
+      match l with 
+      | nil => true
+      | _ => false
+      end)
+    (*combine*)
+    (fun fhd ftl =>
+      fun l => match l with
+                | hd1 :: tl1 => fhd hd1 && ftl tl1
+                | _ => false
+      end)) t1 t2.*)
+From Equations Require Import Equations.
+Section TestEq.
+
+Variable (f: tvsymbol -> ty).
+(*Let's try with Equations and see how the resulting OCaml code is*)
+Equations ty_v_map' (t: ty) : ty by
+  struct t
+  (*wf (ty_size t) lt*) :=
+  ty_v_map' t := ty_v_map_node t.(ty_node)
+where ty_v_map_node (t: ty_node_) : ty by
+  struct t
+  (*wf (ty_node_size t) lt*) :=
+  ty_v_map_node (Tyvar v) := f v;
+  ty_v_map_node (Tyapp ts tys) :=
+    Build_ty_ _ (Tyapp ts (List.map (ty_v_map') tys)) xH.
+
+
+    ty_app f (List.map (ty_v_map fn) tl)
+
+
+  (list ty) (fun v => f v)
+  (fun ts tys res => Build_ty_ _ (Tyapp ts res) xH) 
+  nil cons t.
+
+
+
+ty_v_map (f: tvsymbol -> ty) (t: ty) : ty :=
+  ty_build_simpl ty (list ty) (fun v => f v)
+  (fun ts tys res => Build_ty_ _ (Tyapp ts res) xH) 
+  nil cons t.
+    
+    ) (fun )
+
+
+  (fun ts tys res => res)
+
+(*Now let's try a 2-argument one, of the form:
+  let rec foo (t1 t2: ty) =
+  match t1.ty_node, t2.ty_node with
+  | Tyvar v1, Tyvar v2 => f1 v1 v2
+  | Tyapp ts1 tys1, Tyapp ts2 tys2 => f2 ts1 tys1 ts2 tys2
+  *)
+
+
+(*Writing functions on types*)
+
+(*Decidable equality on types*)
+
 
 
 (*TODO: not best way*)
@@ -63,10 +633,7 @@ Record tvsymbol := {
   tv_name : ident
 }.
 
-(*TODO: add range and float*)
-Inductive type_def (A: Set) : Set :=
-  | NoDef
-  | Alias: A -> type_def A.
+
 
 (*Unset Elimination Schemes.
 Inductive tysymbol : Set :=
@@ -85,35 +652,7 @@ ty_node__ind := Induction for ty_node_ Sort Prop.
 Check ty_ind.*)
 
 
-(*We do this to get around the restriction that
-  Coq Records and Inductives cannot be mutually recursive
-  with each other. TODO: see if we can ensure that
-  this satisfies the correct .mli file*)
-Inductive ty_ (A: Set) : Set := 
-  { ty_node: A;
-    ty_tag: tag}.
 
-Arguments ty_ {A}.
-Arguments ty_node {A}.
-Arguments ty_tag {A}.
-
-Record tysymbol_ (A: Set) : Set := {
-  ts_name : ident;
-  ts_args : list tvsymbol;
-  ts_def : type_def (@ty_ A)
-}.
-
-Arguments tysymbol_ {A}.
-Arguments ts_name {A}.
-Arguments ts_args {A}.
-Arguments ts_def {A}.
-
-Inductive ty_node_ : Set :=
-  | Tyvar : tvsymbol -> ty_node_
-  | Tyapp : @tysymbol_ ty_node_ -> list (@ty_ ty_node_) -> ty_node_.
-
-Definition ty : Set := @ty_ ty_node_.
-Definition tysymbol : Set := @tysymbol_ ty_node_.
 
 (*Test*)
 
@@ -198,41 +737,6 @@ Fail Inductive bad : Set :=
 
 (*Next: structural recursion on size*)
 
-(*TODO: try with Xavier trick (Equations bad extraction I think) and manual rec*)
-(*Define size*)
-Fixpoint ty_node_size (t: ty_node_) : nat :=
-  match t with
-  | Tyvar v => 1
-  | Tyapp ts tys => 1 +
-    (*tysymbol size*)
-    (1 + match (ts_def ts) with
-          | NoDef _ => 0
-          | Alias _ x => 1 + (1 + ty_node_size (x.(ty_node)))
-    end) +
-  
-   list_sum 
-      (map (fun (x: ty) => 1 + ty_node_size (x.(ty_node))) tys)
-  end.
-
-Definition ty_size (t: ty) : nat :=
-  1 + ty_node_size (t.(ty_node)).
-
-Definition tysymbol_size (ts: tysymbol) : nat :=
-  1 + match ts_def ts with
-    | NoDef _ => 0
-    | Alias _ x => 1 + ty_size x
-  end.
-
-Lemma ty_node_size_rewrite (t: ty_node_) :
-  ty_node_size t =
-  match t with
-  | Tyvar v => 1
-  | Tyapp ts tys => 1 + tysymbol_size ts + 
-    list_sum (map ty_size tys)
-  end.
-Proof.
-  destruct t; simpl; auto.
-Qed.
 
 (*Need version of map2 with in*)
 Definition map2' {A B C: Type} :=
@@ -269,11 +773,7 @@ Definition type_def_size (t: type_def ty) : nat :=
 
 
 (*Obligations (do here to test OCaml)*)
-Lemma node_lt_ty (t: ty):
-  ty_node_size (ty_node t) < ty_size t.
-Proof.
-  unfold ty_size. lia.
-Qed.
+
 
 Lemma ty_decomp (t: ty):
 {| ty_node := ty_node t; ty_tag := ty_tag t |} = t.
@@ -281,12 +781,6 @@ Proof.
   destruct t; reflexivity.
 Qed.
 
-Lemma typesym_lt_node (ts: tysymbol) (tys: list ty):
-  tysymbol_size ts < ty_node_size (Tyapp ts tys).
-Proof.
-  rewrite ty_node_size_rewrite.
-  lia.
-Qed.
 
 (*Lemma foo (x: nat) x < x + 1.
 
@@ -376,102 +870,8 @@ Definition tysymbol_ind (ts: tysymbol) : P2 ts := tysymbol_ind' ts (lt_wf _).
 
 End TyInd.
 
-(*Do same with Type so that we can write functions and test extraction*)
-
-Definition type_def_p_ty (P: ty -> Type) (t: type_def ty_) : Type :=
-  match t with
-  | NoDef _ => True
-  | Alias _ x => P x
-  end.
 
 
-Inductive ForallT {A: Type} (P: A -> Type) : list A -> Type :=
-  | ForallT_nil: ForallT P nil
-  | ForallT_cons: forall {x: A} {l: list A},
-    P x -> ForallT P l -> ForallT P (x :: l).
-
-Lemma ForallT_hd {A: Type} (P: A -> Type) (x: A) (l: list A):
-  ForallT P (x :: l) ->
-  P x.
-Proof.
-  intros. inversion X; subst. apply X0.
-Qed.
-
-Lemma ForallT_tl {A: Type} (P: A -> Type) (x: A) (l: list A):
-  ForallT P (x :: l) ->
-  ForallT P l.
-Proof.
-  intros. inversion X; auto.
-Qed.
-
-Lemma ForallT_In {A: Type} (P: A -> Type)
-  (eq_dec: forall (x y: A), {x = y} + {x <> y}) (l: list A):
-  ForallT P l ->
-  forall x, In x l -> P x.
-Proof.
-  intros Hall. induction Hall; simpl; intros.
-  destruct H.
-  destruct (eq_dec x x0); subst; auto.
-  apply IHHall. destruct H; subst; auto.
-  contradiction.
-Qed.
-
-Section TyRect.
-
-Variable (P: ty -> Type).
-Variable (P1: ty_node_ -> Type).
-Variable (P2: tysymbol -> Type).
-
-Variable (Hty: forall (t: ty), P1 (t.(ty_node)) -> P t).
-Variable (Hsym: forall (ts: tysymbol), type_def_p_ty P (ts.(ts_def)) ->
-  P2 ts).
-Variable (Hvar: forall v, P1 (Tyvar v)).
-Variable (Happ: forall ts tys, P2 ts -> ForallT P tys -> P1 (Tyapp ts tys)).
-
-(*This does NOT work - tysymbol is not recursive so we can't have
-  a fixpoint on it
-  Maybe could do same trick (assume we have proof, populate later)
-  but likely to run into positivity problems*)
-
-
-(*Fixpoint gcd_rec (a b: nat) (ACC: Acc lt b) {struct ACC} : nat :=
-  if Nat.eq_dec b 0 then a else gcd_rec b (a mod b) (Acc_inv ACC _).*)
-
-(*TODO: need decomposition if we want idiomatic code, maybe need eq_rect*)
-(*Plan: prove lemmas, do in Set, test extraction (without Program) *)
-Fixpoint ty_rect' (t: ty) (ACC: Acc lt (ty_size t)) {struct ACC} : P t :=
-  (Hty t (ty_node_rect' t.(ty_node) 
-    (Acc_inv ACC (ty_node_size (ty_node t)) (node_lt_ty t))))
-with ty_node_rect' (t: ty_node_) (ACC: Acc lt (ty_node_size t)) {struct ACC} : P1 t :=
-  match t as t' return Acc lt (ty_node_size t') -> P1 t' with
-  | Tyvar tv => fun _ => Hvar tv
-  | Tyapp ts tys => fun ACC => Happ ts tys (tysymbol_rect' ts (Acc_inv ACC (tysymbol_size ts) 
-      (typesym_lt_node ts tys))) 
-    ((fix tys_rect (l: list ty) 
-      (Hl: Forall (fun x => ty_size x < (ty_node_size (Tyapp ts tys))) l) 
-      : ForallT P l :=
-      match l as l' return Forall  (fun x => ty_size x < (ty_node_size (Tyapp ts tys))) l'->
-        ForallT P l'  with
-      | nil => fun _ => ForallT_nil _
-      | x :: xs => fun Hl => ForallT_cons _ (ty_rect' x (Acc_inv ACC (ty_size x) 
-        (List.Forall_inv Hl))) 
-        (tys_rect xs (List.Forall_inv_tail Hl))
-      end Hl) tys (in_tys_lt_app ts tys))
-  end ACC
-with tysymbol_rect' (ts: tysymbol) (ACC: Acc lt (tysymbol_size ts)) {struct ACC} : P2 ts :=
-  Hsym ts (
-    match (ts.(ts_def)) as d' return type_def_size d' < tysymbol_size ts -> 
-       type_def_p_ty P d' with
-    | NoDef _ => fun _ => I
-    | Alias _ x => fun Hlt => ty_rect' x (Acc_inv ACC (ty_size x) (alias_lt_sym Hlt))
-    end (def_lt_sym ts)
-  ).
-
-Definition ty_rect (t: ty) : P t := ty_rect' t (lt_wf _).
-Definition ty_node_rect (t: ty_node_) : P1 t := ty_node_rect' t (lt_wf _).
-Definition tysymbol_rect (ts: tysymbol) : P2 ts := tysymbol_rect' ts (lt_wf _).
-
-End TyRect.
 
 (*Alternate version, more useful*)
 Section TyBuild.
@@ -512,135 +912,11 @@ with ty_node_build' (t: ty_node_) (ACC: Acc lt (ty_node_size t)) {struct ACC} : 
 Definition ty_build (t: ty) := ty_build' t (lt_wf _).
 Definition ty_node_build (t: ty_node_) := ty_node_build' t (lt_wf _).
 
-(*Hmm instead should do*)
-Definition ty_size_rel (t1 t2: ty) : Prop :=
-  ty_size t1 < ty_size t2.
-
-Require Import Coq.Wellfounded.Inverse_Image.
-
-Lemma ty_size_rel_wf: well_founded ty_size_rel.
-Proof.
-  unfold wf. intros.
-  unfold ty_size_rel.
-  apply Inverse_Image.Acc_inverse_image.
-  apply lt_wf.
-Qed.
 
 End TyBuild.
 
-Lemma in_tys_lt_app' {t ts tys}:
-  ty_node_size (Tyapp ts tys) < ty_size t ->
-  Forall (fun x => ty_size_rel x t) tys.
-Proof.
-  rewrite ty_node_size_rewrite. intros.
-  intros.
-  rewrite List.Forall_forall; intros x Hinx.
-  unfold ty_size_rel.
-  pose proof (in_split x tys Hinx) as Hsplit.
-  destruct Hsplit as [l1 [l2 Htys]]; subst.
-  revert H.
-  rewrite map_app. simpl map.
-  rewrite list_sum_app. simpl list_sum.
-  intros.
-  unfold ty_size at 1. lia.
-Qed.
+
   
-Section TyBuildSimpl.
-
-Variable (A: Type)(B: Type).
-
-Variable (Hvar: tvsymbol -> A).
-Variable (Happ: tysymbol -> list ty -> B -> A).
-
-Variable (base: B).
-Variable (combine: A -> B -> B).
-
-Fixpoint ty_build_simpl' (t: ty) (ACC: Acc ty_size_rel t) {struct ACC} : A :=
-  match t.(ty_node) as n return ty_node_size n < ty_size t -> A with
-  | Tyvar v => fun _ => Hvar v
-  | Tyapp ts tys => fun Hlt => Happ ts tys
-    ((fix tys_fold (l: list ty) (Hall: Forall (fun x => ty_size_rel x t) l) : B :=
-      match l as l' return Forall (fun x => ty_size_rel x t) l' -> B with
-      | nil => fun _ => base
-      | x :: xs => fun Hall => 
-        combine (ty_build_simpl' x (Acc_inv ACC _ (Forall_inv Hall))) 
-        (tys_fold xs (Forall_inv_tail Hall))
-      end Hall) tys (in_tys_lt_app'  Hlt))
-  end (node_lt_ty t).
-
-Definition ty_build_simpl t := ty_build_simpl' t (ty_size_rel_wf t).
-
-(*This is what we need*)
-Definition ty_node_size_rel (t1 t2: ty) : Prop :=
-  ty_node_size (t1.(ty_node)) < ty_node_size (t2.(ty_node)).
-
-Lemma ty_node_size_rel_wf: well_founded ty_node_size_rel.
-Proof.
-  unfold wf. intros.
-  unfold ty_node_size_rel.
-  apply Inverse_Image.Acc_inverse_image.
-  apply lt_wf.
-Qed.
-
-Lemma ty_size_rel_node_rel (t1 t2: ty):
-  ty_size_rel t1 t2 <-> ty_node_size_rel t1 t2.
-Proof.
-  unfold ty_size_rel, ty_size, ty_node_size_rel. lia.
-Qed.
-
-
-Lemma ty_build_simpl_irrel t ACC1 ACC2:
-  ty_build_simpl' t ACC1 = ty_build_simpl' t ACC2.
-Proof.
-  induction t using (well_founded_induction ty_node_size_rel_wf).
-  destruct ACC1; destruct ACC2.
-  simpl.
-  destruct t as [n tg]; simpl. destruct n; auto.
-  f_equal.
-  generalize dependent (in_tys_lt_app' (node_lt_ty {| ty_node := Tyapp t l; ty_tag := tg |})).
-  (*assert (ty_size {| ty_node := Tyapp t l; ty_tag := tg |} <= )*)
-  generalize dependent {| ty_node := Tyapp t l; ty_tag := tg |}.
-  induction l; simpl; auto.
-  intros. erewrite IHl. f_equal.
-  apply H.
-  inversion f; subst.
-  apply ty_size_rel_node_rel. auto.
-  auto.
-Qed.
-
-
-
-
-
-Lemma ty_build_simpl_rewrite (t: ty) :
-  ty_build_simpl t =
-  match t.(ty_node) with
-        | Tyvar v => Hvar v
-        | Tyapp ts tys => Happ ts tys 
-            (fold_right (fun x acc => combine (ty_build_simpl x) acc) base tys)
-  end.
-Proof.
-  unfold ty_build_simpl at 1.
-  generalize dependent (ty_size_rel_wf t).
-  intros a. destruct a.
-  destruct t as [n tg].
-  destruct n; [reflexivity |].
-  simpl. f_equal.
-  (*Problem: have l in Forall*)
-  generalize dependent (in_tys_lt_app' (node_lt_ty {| ty_node := Tyapp t l; ty_tag := tg |})).
-  (*assert (ty_size {| ty_node := Tyapp t l; ty_tag := tg |} <= )*)
-  generalize dependent {| ty_node := Tyapp t l; ty_tag := tg |}.
-  intros t' a'.
-  (*TODO: see if we need size info*)
-  induction l; simpl; auto.
-  intros.
-  rewrite IHl.
-  f_equal.
-  apply ty_build_simpl_irrel.
-Qed.
-
-End TyBuildSimpl.
-
 
 
 (*TODO: prove this later*)
@@ -764,15 +1040,7 @@ end ).
 
 End TyBuild.*)
 
-Definition ty_v_map (f: tvsymbol -> ty) (t: ty) : ty :=
-  ty_build_simpl ty (list ty) (fun v => f v)
-  (fun ts tys res => Build_ty_ _ (Tyapp ts res) xH) 
-  nil cons t.
 
-Definition ty_v_map' (f: tvsymbol -> ty) (t: ty) : ty :=
-  ty_build ty ty (list ty) (fun _ x => x) (fun v => f v)
-  nil (fun acc x => x :: acc) (fun ts tys res => 
-    Build_ty_ _ (Tyapp ts res) xH) t.
 
 
 (*
@@ -1053,3 +1321,4 @@ Definition ts_equal (t1 t2: tysymbol) : bool :=
 
 
 
+*)
