src/util/CoqBigInt.v
@@ -1,0 +1,116 @@
+(*Here, we axiomatize OCaml's big ints (Z.t) in Coq.
+  We provide 2 different types, one for nonnegative ints
+  and one for general ints (which we need less)*)
+(*TODO: add general: for now, just positive*)
+Require Export Coq.ZArith.BinInt.
+Require Export CoqInt.
+
+Axiom t : Type.
+Axiom one : t.
+Axiom zero : t.
+Axiom add : t -> t -> t.
+Axiom succ : t -> t.
+Axiom eq : t -> t -> bool.
+Axiom compare: t -> t -> int.
+
+(*Assumption: equality corresponds to Leibnitz equality*)
+Axiom eq_spec : forall (x y: t), x = y <-> eq x y = true.
+
+Axiom to_pos : t -> positive.
+(*OCaml function to_pos - gives positive of (x+1) because
+  we allow 0 values
+  (*Go from [numbits x]-1 down to 0*)
+  let to_pos (x: Z.t) = 
+    let rec build_pos (n: int) (x: Z.t) (base: positive) : positive =
+      if n < 0 then base else
+      let b = Z.testbit x n in
+      if b then build_pos (n-1) (xI base)
+      else build_pos (n-1) (xO base)
+    in build_pos (Z.numbits x - 2) (Z.succ x) xH
+*)
+(*NOTE: this is true ONLY because we only consider nonnegative
+  values
+  TODO: implement to_pos with primitives, prove this*)
+Axiom to_pos_inj: forall (x y: t), to_pos x = to_pos y -> x = y.
+
+(*This one we can implement in Coq (TODO)*)
+Axiom of_pos : positive -> t.
+
+(*TODO: general ints*)
+
+
+
+(*Instead of the standard library, which uses modules, we use a
+  record which can be instantiated either with Z/positive 
+  (for computation inside of Coq) or with OCaml Z.t*)
+(*Require Export Coq.ZArith.BinInt.
+(*The operations a type must have for it to be
+  a "BigInt"*)
+Record BigIntTy (A: Type) := {
+  big_int_zero : A;
+  big_int_one: A;
+  big_int_succ: A -> A;
+  big_int_add : A -> A -> A;
+  big_int_eq : A -> A -> bool
+}.
+
+Definition BigInt_Z : BigIntTy Z := 
+{|big_int_zero := 0%Z; big_int_one := 1%Z; big_int_succ := Z.succ;
+big_int_add := Z.add; big_int_eq := Z.eqb|}.
+
+(*Not quite right: BigInt is module, t is type*)
+(*We just want a type along with operations
+  (i.e. field should be type, NOT module )*)
+
+(*How do they extract module currentlY?
+  Probably - extract to module type, implement with Big_int 
+    (manually)
+  what we want - maybe just axioms
+  But then we cannot instantiate with Z, right?
+  Is it so important to instantiate with Z?
+  Would be nice*)
+(*Instead, what we want is this:
+  Axiom obigint : Type
+  *)
+(*Idea: extract BigInt to BigInt.t
+  extract t to BigInt.t (really, really bad)
+  extract zero to BigInt.zero*)
+(*Maybe typeclass? Say that a type has property BigInt
+  if it contains all the needed functions?
+  But problem is that this is axiom - instead, we want to
+  have each as axioms that can be instantiated (or defined)
+  separately*)
+(*For now, axiomatize?*)
+(*basically, record/typeclass of functions should work, but
+  then we have to instantiate
+  
+  AHA, this is how we will do it (clunkily) *)
+
+(*Not the most elegant but OK*)
+
+(*Axiomatize OCaml BigInts for now
+  TODO: see if nice way to abstract (without modules)
+  *)
+Axiom t : Type.
+Axiom one : t.
+Axiom zero : t.
+Axiom add : t -> t -> t.
+Axiom succ : t -> t.
+Axiom eq : t -> t -> bool.
+
+(*Assumption: equality corresponds to Leibnitz equality*)
+Axiom eq_spec : forall (x y: t), x = y <-> eq x y = true.
+
+(*We will write this function in OCaml (TODO)*)
+Axiom to_Z : t -> Z.
+(*Question: how to deal with positive values?
+  Should we have 2 types in Coq, extract both to OCaml big_int?
+  maybe
+  TODO: start*)
+
+Definition OcamlBigInt : BigIntTy t := 
+{|big_int_zero := zero; big_int_one := one;
+  big_int_succ := succ; big_int_add := add;
+  big_int_eq := eq|}.
+
+  *)
