src/util/CoqInt.v
@@ -1,0 +1,8 @@
+(*A light axiomatization of OCaml ints. We really don't need
+  very much*)
+(*Here, we use bounded ints so that we can extract directly
+  to OCaml's int type*)
+Parameter int : Type.
+Parameter int_eqb : int -> int -> bool.
+(*Parameter Abs : int -> Z.*)
+Parameter int_eqb_eq: forall (i1 i2: int), i1 = i2 <-> int_eqb i1 i2 = true.
