src/util/Number.v
@@ -1,0 +1,16 @@
+(*Why3 Number uses BigInt; we will use Z*)
+Require CoqBigInt.
+
+(** Range checks *)
+Record int_range := {
+  ir_lower : CoqBigInt.t;
+  ir_upper : CoqBigInt.t
+}.
+
+Definition create_range lo hi : int_range :=
+  {| ir_lower := lo; ir_upper := hi|}.
+
+Record float_format := {
+  fp_exponent_digits : CoqBigInt.t;
+  fp_significand_digits : CoqBigInt.t 
+}.
