src/util/StateMonad.v
@@ -1,0 +1,97 @@
+(*A mutable counter to register identifiers*)
+Require CoqBigInt.
+
+(*We offer a restricted subset of the state monad interface
+  so that we can extract to OCaml mutable references soundly*)
+Definition ctr (a: Type) : Type := CoqBigInt.t -> CoqBigInt.t * a.
+
+(*Note: should not be used directly*)
+Definition ctr_get : ctr CoqBigInt.t := fun x => (x, x).
+
+Definition ctr_ret {a: Type} (x: a) : ctr a := fun s => (s, x).
+Definition ctr_bnd {a b: Type} (f: a -> ctr b) (x: ctr a) : ctr b :=
+  fun i =>
+    let t := x i in
+    f (snd t) (fst t).
+
+Definition new_ctr : ctr unit := fun _ => (CoqBigInt.zero, tt).
+Definition incr : ctr unit := fun i => (CoqBigInt.succ i, tt).
+
+From stdpp Require Import base.
+Global Instance ctr_ret': MRet ctr := @ctr_ret.
+Global Instance ctr_bnd': MBind ctr := @ctr_bnd.
+
+
+(*Definition st_bnd {s a b: Type} (f: a -> state s b) (x: state s a) : state s b :=
+  fun s => 
+    let t := runState x s in
+    runState (f (snd t)) (fst t).
+
+
+Definition ctr_bind
+
+
+(*We want a mutable counter to register identifiers*)
+
+(*We offer a very restricted interface so that we can
+  extract to OCaml mutable references soundly*)
+
+Definition state (s: Type) (a: Type) : Type := s -> s * a.
+Definition runState {s a} (x: state s a) : s -> s * a := x.
+
+Definition st_ret {s a} (x: a) : state s a :=
+  fun s => (s, x).
+
+Definition get {s: Type} : state s s :=
+  fun s => (s, s).
+Definition put {s: Type} (x: s) : state s unit :=
+  fun _ => (x, tt).
+Definition evalState {s a: Type} (x: state s a) (y: s) : a :=
+  snd (x y).
+Definition execState {s a: Type} (x: state s a) (y: s) : s :=
+  fst (x y).
+
+Definition st_bnd {s a b: Type} (f: a -> state s b) (x: state s a) : state s b :=
+  fun s => 
+    let t := runState x s in
+    runState (f (snd t)) (fst t).
+
+From stdpp Require Import base.
+Global Instance state_ret {s: Type}: MRet (state s) := @st_ret s.
+Global Instance errorM_bind {s: Type}: MBind (state s) := @st_bnd s.
+
+
+(*For now, only 1 global counter/int that is stored
+  TODO: see if we need others*)
+Require CoqBigInt.
+Definition ctr (a: Type) := state CoqBigInt.t a.
+Definition new_ctr {a: Type} (i: CoqBigInt.t) (x: a) : ctr a :=
+  fun _ => (i, x).
+Definition incr : ctr unit :=
+  fun i => (CoqBigInt.succ i, tt).
+  (*ONLY through this interface!*)
+  
+
+
+
+
+
+(*Axiom ST : Type -> Type -> Type.
+Axiom runST : forall (a: Type), (forall s, ST s a) -> a.
+Axiom bnd : forall (s a b: Type), ST s a -> (a -> ST s b) -> ST s b.
+Axiom ret: forall (s a: Type), a -> ST s a.
+
+Axiom STRef : Type -> Type -> Type.
+Axiom newSTRef : forall (s a: Type), a -> ST s (STRef s a).
+Axiom readSTRef : forall (s a: Type), STRef s a -> ST s a.
+Axiom writeSTRef: forall (s a: Type), STRef s a -> a -> ST s unit.
+Axiom modifySTRef: forall (s a: Type), STRef s a -> (a -> a) -> ST s unit.
+
+(*A counter*)
+Require CoqBigInt.
+Definition new_ctr (s: Type) : ST s (STRef s CoqBigInt.t) :=
+  newSTRef s _ (CoqBigInt.zero).
+Definition incr (s: Type) (ctr: STRef s CoqBigInt.t) : 
+  ST s (STRef s CoqBigInt.t) :=
+  modifySTRef _ _ ctr CoqBigInt.succ.
+  bnd _ _ _ ctr (fun x => ret _ _ (CoqBigInt.succ x)).*)*)
